Some refactoring, more proofs on insert and result

thys/MFODL_Monitor_Devel/Optimized_Agg.thy
@@ -1,113 +1,456 @@
 theory Optimized_Agg
   imports Monitor
 begin
+
 type_synonym 'a agg_map = "(event_data tuple, 'a) mapping"
 
-datatype aggaux = CntAux "int agg_map" | SumAux "event_data table" | MinAux "event_data table"
-                    | MaxAux "event_data table" | AvgAux "event_data table" | MedAux "event_data table"
+datatype aggaux' = CntAux nat
+
+datatype aggaux = CntAux "nat agg_map" | SumAux "(nat \<times> event_data) agg_map" | MinAux "event_data table"
+  | MaxAux "event_data table" | MedAux "event_data table"
+
+definition group_multiset where
+  "group_multiset k b f X = (let group = Set.filter (\<lambda>x. drop b x = k) X in
+                      (\<lambda>y. (y, ecard (Set.filter (\<lambda>x. meval_trm f x = y) group))) ` meval_trm f ` group)"
+
+definition valid_aggmap :: "(event_data list \<Rightarrow> 'a) \<Rightarrow> nat \<Rightarrow> Formula.trm \<Rightarrow> (event_data option list, 'a) mapping \<Rightarrow> event_data option list set \<Rightarrow> bool" where
+  "valid_aggmap g b f m X \<longleftrightarrow> (\<forall>k. k \<in> (drop b) ` X \<longleftrightarrow> k \<in> Mapping.keys m) \<and>
+                    (\<forall>k. k \<in> Mapping.keys m \<longrightarrow> Mapping.lookup m k = 
+                    (let M = group_multiset k b f X
+                    in Some (g (flatten_multiset M))))"
 
 fun valid_maggaux :: "aggargs \<Rightarrow> aggaux \<Rightarrow> event_data table \<Rightarrow> bool" where
-  "valid_maggaux \<lparr>aggargs_cols = cols, aggargs_n = n, aggargs_g0 = g0, aggargs_y = y, aggargs_\<omega> = \<omega>, aggargs_b = b, aggargs_f = f\<rparr> aux data = 
+  "valid_maggaux \<lparr>aggargs_cols = cols, aggargs_n = n, aggargs_g0 = g0, aggargs_y = y, aggargs_\<omega> = \<omega>, aggargs_b = b, aggargs_f = f\<rparr> aux X = 
+  (finite X \<and>
   (let aggtype = fst \<omega> in case aux of 
       CntAux m \<Rightarrow>
-        (aggtype = Formula.Agg_Cnt) \<and> (data = {} \<longleftrightarrow> Mapping.keys m = {}) \<and>
-        (\<forall>k. k \<in> (drop b) ` data \<longleftrightarrow> k \<in> Mapping.keys m) \<and>
-        (\<forall>k. k \<in> Mapping.keys m \<longrightarrow> Mapping.lookup m k = 
-          (let group = Set.filter (\<lambda>x. drop b x = k) data;
-           M = (\<lambda>y. (y, ecard (Set.filter (\<lambda>x. meval_trm f x = y) group))) ` meval_trm f ` group
-          in Some (length (flatten_multiset M))))
-    | SumAux t \<Rightarrow> (aggtype = Formula.Agg_Sum) \<and> t = data
-    | MinAux t \<Rightarrow> (aggtype = Formula.Agg_Min) \<and> t = data
-    | MaxAux t \<Rightarrow> (aggtype = Formula.Agg_Max) \<and> t = data
-    | AvgAux t \<Rightarrow> (aggtype = Formula.Agg_Avg) \<and> t = data
-    | MedAux t \<Rightarrow> (aggtype = Formula.Agg_Med) \<and> t = data)"
+        (aggtype = Formula.Agg_Cnt) \<and> 
+        (valid_aggmap (\<lambda>k. length k) b f m X)
+    | SumAux m \<Rightarrow> (aggtype = Formula.Agg_Sum \<or> aggtype = Formula.Agg_Avg) \<and> 
+                  (let y0 = (if aggtype = Formula.Agg_Sum then snd \<omega> else EInt 0) in
+                  (valid_aggmap (\<lambda>k. (length k, foldl plus y0 k)) b f m X))
+    | MinAux t \<Rightarrow> (aggtype = Formula.Agg_Min) \<and> t = X
+    | MaxAux t \<Rightarrow> (aggtype = Formula.Agg_Max) \<and> t = X
+    | MedAux t \<Rightarrow> (aggtype = Formula.Agg_Med) \<and> t = X))"
 
 fun init_maggaux :: "aggargs \<Rightarrow> aggaux" where
   "init_maggaux args =
   (let aggtype = fst (aggargs_\<omega> args) in case aggtype of
       Formula.Agg_Cnt \<Rightarrow> CntAux Mapping.empty
-    | Formula.Agg_Sum \<Rightarrow> SumAux {}
+    | Formula.Agg_Sum \<Rightarrow> SumAux Mapping.empty
     | Formula.Agg_Min \<Rightarrow> MinAux {}
     | Formula.Agg_Max \<Rightarrow> MaxAux {}
-    | Formula.Agg_Avg \<Rightarrow> AvgAux {}
+    | Formula.Agg_Avg \<Rightarrow> SumAux Mapping.empty
     | Formula.Agg_Med \<Rightarrow> MedAux {})"
 
+fun insert_cnt :: "aggargs \<Rightarrow> nat agg_map \<Rightarrow> event_data tuple \<Rightarrow> nat agg_map" where
+  "insert_cnt args m t = (let group = drop (aggargs_b args) t 
+                       in case (Mapping.lookup m group) of
+                        Some i \<Rightarrow> Mapping.update group (i + 1) m
+                      | None \<Rightarrow> Mapping.update group 1 m)"
+
+fun insert_sum :: "aggargs \<Rightarrow> event_data \<Rightarrow> (nat \<times> event_data) agg_map \<Rightarrow> event_data tuple \<Rightarrow> (nat \<times> event_data) agg_map" where
+  "insert_sum args y0 m t = (let group = drop (aggargs_b args) t;
+                                         term = meval_trm (aggargs_f args) t
+                                     in case (Mapping.lookup m group) of
+                        Some (cnt, agg_sum) \<Rightarrow> Mapping.update group (cnt + 1, agg_sum + term) m
+                      | None \<Rightarrow> Mapping.update group (1, y0 + term) m)"
+
 fun insert_maggaux :: "aggargs \<Rightarrow> event_data table \<Rightarrow> aggaux \<Rightarrow> aggaux" where
-  "insert_maggaux  \<lparr>aggargs_cols = cols, aggargs_n = n, aggargs_g0 = g0, aggargs_y = y, aggargs_\<omega> = \<omega>, aggargs_b = b, aggargs_f = f\<rparr> data aux = (case aux of
-    CntAux m \<Rightarrow> CntAux (foldl (\<lambda> m t. (let group = drop b t in case (Mapping.lookup m group) of
-                                       Some i \<Rightarrow> Mapping.update group (i + 1) m
-                                       | None \<Rightarrow> Mapping.update group 1 m) ) m (csorted_list_of_set data))
-  | SumAux t \<Rightarrow> SumAux (t \<union> data)
+  "insert_maggaux args data aux = (case aux of
+    CntAux m \<Rightarrow> CntAux (foldl (insert_cnt args) m (csorted_list_of_set data))
+  | SumAux m \<Rightarrow> let y0 = snd (aggargs_\<omega> args) in SumAux (foldl (insert_sum args y0) m (csorted_list_of_set data))
   | MinAux t \<Rightarrow> MinAux (t \<union> data)
   | MaxAux t \<Rightarrow> MaxAux (t \<union> data)
-  | AvgAux t \<Rightarrow> AvgAux (t \<union> data)
   | MedAux t \<Rightarrow> MedAux (t \<union> data))"
 
+fun delete_cnt :: "nat \<Rightarrow> nat agg_map \<Rightarrow> event_data tuple \<Rightarrow> nat agg_map" where
+  "delete_cnt b m t = (let group = drop b t
+                       in case (Mapping.lookup m group) of
+                         Some i \<Rightarrow> (if i = 1 then Mapping.delete group m 
+                                    else Mapping.update group (i - 1) m)
+                       | None \<Rightarrow> m)"
+
+fun delete_sum :: "aggargs \<Rightarrow> (nat \<times> event_data) agg_map \<Rightarrow> event_data tuple \<Rightarrow> (nat \<times> event_data) agg_map" where
+  "delete_sum args m t = (let group = drop (aggargs_b args) t;
+                              term = meval_trm (aggargs_f args) t
+                          in case (Mapping.lookup m group) of
+                            Some (cnt, agg_sum) \<Rightarrow> (if cnt = 1 then Mapping.delete group m
+                                                    else Mapping.update group (cnt - 1, agg_sum - term) m)
+                          | None \<Rightarrow> m)"
+
 fun delete_maggaux :: "aggargs \<Rightarrow> event_data table \<Rightarrow> aggaux \<Rightarrow> aggaux" where
-  "delete_maggaux  \<lparr>aggargs_cols = cols, aggargs_n = n, aggargs_g0 = g0, aggargs_y = y, aggargs_\<omega> = \<omega>, aggargs_b = b, aggargs_f = f\<rparr> data aux = (case aux of
-    CntAux m \<Rightarrow> CntAux (foldl (\<lambda> m t. (let group = drop b t in case (Mapping.lookup m group) of
-                                       Some i \<Rightarrow> (if i = 1 then Mapping.delete group m 
-                                                  else Mapping.update group (i - 1) m)
-                                       | None \<Rightarrow> m) ) m (csorted_list_of_set data))
-  | SumAux t \<Rightarrow> SumAux (t - data)
+  "delete_maggaux args data aux = (case aux of
+    CntAux m \<Rightarrow> CntAux (foldl (delete_cnt (aggargs_b args)) m (csorted_list_of_set data))
+  | SumAux m \<Rightarrow> SumAux (foldl (delete_sum args) m (csorted_list_of_set data))
   | MinAux t \<Rightarrow> MinAux (t - data)
   | MaxAux t \<Rightarrow> MaxAux (t - data)
-  | AvgAux t \<Rightarrow> AvgAux (t - data)
   | MedAux t \<Rightarrow> MedAux (t - data))"
 
 fun result_maggaux :: "aggargs \<Rightarrow> aggaux \<Rightarrow> event_data table" where
   "result_maggaux \<lparr>aggargs_cols = cols, aggargs_n = n, aggargs_g0 = g0, aggargs_y = y, aggargs_\<omega> = \<omega>, aggargs_b = b, aggargs_f = f\<rparr> aux = (case aux of
-    CntAux m \<Rightarrow> (if g0 \<and> Mapping.keys m = {} then singleton_table n y (eval_agg_op \<omega> {})
-    else (\<lambda>k. let agg_val = (EInt (integer_of_int (Mapping.lookup_default 0 m k))) in
-            k[y:=Some agg_val]) ` Mapping.keys m)
-  | SumAux t \<Rightarrow> eval_aggargs \<lparr>aggargs_cols = cols, aggargs_n = n, aggargs_g0 = g0, aggargs_y = y, aggargs_\<omega> = \<omega>, aggargs_b = b, aggargs_f = f\<rparr> t
+    CntAux m \<Rightarrow> (if g0 \<and> Mapping.keys m = {} 
+                then singleton_table n y (eval_agg_op \<omega> {})
+                else (\<lambda>k. (case Mapping.lookup m k of
+                             Some i \<Rightarrow> k[y:=Some (EInt (integer_of_int i))]
+                           | None \<Rightarrow> k))` Mapping.keys m)
+  | SumAux m \<Rightarrow> (if g0 \<and> Mapping.keys m = {}
+                      then singleton_table n y (eval_agg_op \<omega> {})
+                      else if fst \<omega> = Formula.Agg_Sum
+                      then (\<lambda>k. (case Mapping.lookup m k of 
+                                   Some (_, agg_sum) \<Rightarrow> k[y:=Some agg_sum]
+                                 | None \<Rightarrow> k)) ` Mapping.keys m
+                      else (\<lambda>k. (case Mapping.lookup m k of
+                                   Some (cnt, agg_sum) \<Rightarrow> k[y:=Some (EFloat ((double_of_event_data agg_sum) / (double_of_int cnt)))] 
+                                 | None \<Rightarrow> k)) ` Mapping.keys m)
   | MinAux t \<Rightarrow> eval_aggargs \<lparr>aggargs_cols = cols, aggargs_n = n, aggargs_g0 = g0, aggargs_y = y, aggargs_\<omega> = \<omega>, aggargs_b = b, aggargs_f = f\<rparr> t
   | MaxAux t \<Rightarrow> eval_aggargs \<lparr>aggargs_cols = cols, aggargs_n = n, aggargs_g0 = g0, aggargs_y = y, aggargs_\<omega> = \<omega>, aggargs_b = b, aggargs_f = f\<rparr> t
-  | AvgAux t \<Rightarrow> eval_aggargs \<lparr>aggargs_cols = cols, aggargs_n = n, aggargs_g0 = g0, aggargs_y = y, aggargs_\<omega> = \<omega>, aggargs_b = b, aggargs_f = f\<rparr> t
   | MedAux t \<Rightarrow> eval_aggargs \<lparr>aggargs_cols = cols, aggargs_n = n, aggargs_g0 = g0, aggargs_y = y, aggargs_\<omega> = \<omega>, aggargs_b = b, aggargs_f = f\<rparr> t)"
 
 lemma valid_init_maggaux_unfolded: "safe_aggargs \<lparr>aggargs_cols = cols, aggargs_n = n, aggargs_g0 = g0, aggargs_y = y, aggargs_\<omega> = \<omega>, aggargs_b = b, aggargs_f = f\<rparr> \<Longrightarrow> valid_maggaux \<lparr>aggargs_cols = cols, aggargs_n = n, aggargs_g0 = g0, aggargs_y = y, aggargs_\<omega> = \<omega>, aggargs_b = b, aggargs_f = f\<rparr> (init_maggaux \<lparr>aggargs_cols = cols, aggargs_n = n, aggargs_g0 = g0, aggargs_y = y, aggargs_\<omega> = \<omega>, aggargs_b = b, aggargs_f = f\<rparr>) {}"
-  apply(induction "fst \<omega>")
-  by (auto)
+  by (cases "fst \<omega>") (auto simp add:valid_aggmap_def)
 
 lemma valid_init_maggaux: "safe_aggargs args \<Longrightarrow> valid_maggaux args (init_maggaux args) {}"
   using valid_init_maggaux_unfolded by (cases args) fast
 
+primrec iter_f :: "('a \<Rightarrow> 'b \<Rightarrow> 'b) \<Rightarrow> nat \<Rightarrow> 'a \<Rightarrow> 'b \<Rightarrow> 'b"
+  where
+    "iter_f f 0 t y0 = y0"
+  | "iter_f f (Suc n) t y0 = f t (iter_f f n t y0)"
+
+lemma iter_f_comm: 
+  assumes commute_f: "comp_fun_commute f"
+  shows "iter_f f n1 t1 (iter_f f n2 t2 y0) = iter_f f n2 t2 (iter_f f n1 t1 y0)"
+proof(induction n1)
+  case 0
+  then show ?case by auto
+next
+  case (Suc n)
+  then show ?case sorry
+qed
+
+
+lemma fold_flatten_multiset: 
+  assumes finite_m: "finite M"
+  assumes commute_f: "comp_fun_commute f"
+  shows "fold f (flatten_multiset M) y0  = Finite_Set.fold (\<lambda> (t, m) y. iter_f f (the_enat m) t y) y0 M"
+proof -
+  interpret comp_fun_commute "\<lambda> (t, m) y. iter_f f (the_enat m) t y"
+    using iter_f_comm[of f] commute_f
+    by unfold_locales auto
+  obtain c where c_def: "ID ccompare = Some (c :: (event_data \<times> enat) comparator)" 
+    by (simp add: ID_def ccompare_prod_def ccompare_event_data_def ccompare_enat_def split:if_splits option.splits)
+  note c = ID_ccompare'[OF c_def] 
+  note c_class = comparator.linorder[OF c]
+  show ?thesis
+    using finite_m
+  proof(induction M)
+    case empty
+    then show ?case
+      using linorder.sorted_list_of_set_empty[OF c_class]
+      by (auto simp add:flatten_multiset_def csorted_list_of_set_def c_def)
+  next
+    case (insert x F)
+    obtain t m where "x = (t, m)"
+      by (cases x) auto
+    then show ?case
+      using insert(1-2) insert(3)[symmetric] linorder.sorted_list_of_set_insert[OF c_class]
+      apply(simp add:flatten_multiset_def csorted_list_of_set_def c_def) sorry
+  qed
+qed
+
+lemma length_fold: "length xs = fold (\<lambda> _ n. n + 1) xs 0"
+  by (induction xs) (auto simp:fold_commute_apply)
+
+lemma iter_f_len: "iter_f (\<lambda> _. Suc) m t y = y + m"
+  by (induction m) auto
+
+lemma length_flatten_multiset: 
+  assumes "finite M"
+  shows "length (flatten_multiset M) = Finite_Set.fold (\<lambda> (t, m) y. y + (the_enat m)) 0 M"
+  using length_fold[of "flatten_multiset M"] by (simp add: fold_flatten_multiset assms comp_fun_commute.intro iter_f_len)
+
+lemma valid_insert_cnt_unfolded: 
+  assumes valid_before: "valid_maggaux \<lparr>aggargs_cols = cols, aggargs_n = n, aggargs_g0 = g0, aggargs_y = y, aggargs_\<omega> = \<omega>, aggargs_b = b, aggargs_f = f\<rparr> (CntAux m) X" 
+  and correct_type: "type_restr \<lparr>aggargs_cols = cols, aggargs_n = n, aggargs_g0 = g0, aggargs_y = y, aggargs_\<omega> = \<omega>, aggargs_b = b, aggargs_f = f\<rparr> {elem}"
+  and disjoint: "elem \<notin> X"
+shows "valid_maggaux \<lparr>aggargs_cols = cols, aggargs_n = n, aggargs_g0 = g0, aggargs_y = y, aggargs_\<omega> = \<omega>, aggargs_b = b, aggargs_f = f\<rparr> 
+        (CntAux (insert_cnt \<lparr>aggargs_cols = cols, aggargs_n = n, aggargs_g0 = g0, aggargs_y = y, aggargs_\<omega> = \<omega>, aggargs_b = b, aggargs_f = f\<rparr> m elem)) (X \<union> {elem})"
+proof - 
+  define updated_map where "updated_map = insert_cnt \<lparr>aggargs_cols = cols, aggargs_n = n, aggargs_g0 = g0, aggargs_y = y, aggargs_\<omega> = \<omega>, aggargs_b = b, aggargs_f = f\<rparr> m elem"
+  define updated_data where "updated_data = X \<union> {elem}"
+  interpret comp_fun_commute "\<lambda>(t, m) y. y + the_enat m" 
+    by(unfold_locales) auto
+  have valid_finite: "finite updated_data" using valid_before by (auto simp:updated_data_def)
+  have valid_key_invariant: "\<And>k. k \<in> (drop b) ` updated_data \<longleftrightarrow> k \<in> Mapping.keys updated_map"
+  proof (rule iffI)
+    fix k
+    assume assm: "k \<in> (drop b) ` updated_data"
+    show "k \<in>  Mapping.keys updated_map"
+      using valid_before assm
+      unfolding updated_map_def updated_data_def
+      by (cases "k \<in> (drop b) ` X") (auto simp: valid_aggmap_def Let_def split:option.splits)
+  next
+    fix k
+    assume assm: "k \<in> Mapping.keys updated_map"
+    show "k \<in> (drop b) ` updated_data"
+      using valid_before assm
+      unfolding updated_map_def updated_data_def
+      by (cases "k \<in> Mapping.keys m") (auto simp: valid_aggmap_def Let_def split:option.splits)
+  qed
+  have valid_value_invariant: "\<And>k. k \<in> Mapping.keys updated_map \<longrightarrow> Mapping.lookup updated_map k = 
+          (let group = Set.filter (\<lambda>x. drop b x = k) updated_data;
+           M = (\<lambda>y. (y, ecard (Set.filter (\<lambda>x. meval_trm f x = y) group))) ` meval_trm f ` group
+          in Some (length (flatten_multiset M)))"
+  proof rule
+    fix k
+    define group where "group = Set.filter (\<lambda>x. drop b x = k) updated_data"
+    define M where "M = (\<lambda>y. (y, ecard (Set.filter (\<lambda>x. meval_trm f x = y) group))) ` meval_trm f ` group"
+    define old_group where "old_group = Set.filter (\<lambda>x. drop b x = k) X"
+    define old_M where "old_M = (\<lambda>y. (y, ecard (Set.filter (\<lambda>x. meval_trm f x = y) old_group))) ` meval_trm f ` old_group"
+    assume assm: "k \<in> Mapping.keys updated_map"
+    show "Mapping.lookup updated_map k = 
+          (let group = Set.filter (\<lambda>x. drop b x = k) updated_data;
+           M = (\<lambda>y. (y, ecard (Set.filter (\<lambda>x. meval_trm f x = y) group))) ` meval_trm f ` group
+          in Some (length (flatten_multiset M)))"
+    proof (cases "k \<in> Mapping.keys m")
+      case False
+      then have map_val: "Mapping.lookup updated_map k = Some 1" 
+        using assm by (auto simp: updated_map_def keys_is_none_rep Let_def lookup_update' split:option.splits)
+      have "drop b elem = k" 
+        using assm False 
+        by(auto simp: updated_map_def Let_def split:option.splits)
+      then have group_single_elem: "group = {elem}" 
+        using False valid_before image_iff
+        by(fastforce simp: group_def updated_data_def valid_aggmap_def)
+      then have "M = insert (meval_trm f elem, enat 1) {}"
+        using group_single_elem unfolding M_def Set.filter_def ecard_def by (auto cong: conj_cong)
+      then have "length(flatten_multiset M) = 1" 
+        using length_flatten_multiset[of M] Finite_Set.comp_fun_commute.fold_insert by(auto)
+      then show ?thesis using map_val by (simp add: M_def local.group_def)
+    next
+      case True
+      then show ?thesis sorry
+        
+    qed
+  qed
+  show ?thesis using valid_value_invariant valid_key_invariant valid_finite valid_before
+    by (auto simp add:updated_data_def valid_aggmap_def updated_map_def group_multiset_def Let_def)
+qed
+
+lemma valid_aggmap_empty_data: "valid_aggmap g b f m X \<Longrightarrow> X = {} \<longleftrightarrow> Mapping.keys m = {}"
+  by (auto simp:valid_aggmap_def)
+
+lemma flatten_multiset_not_empty: 
+  assumes valid_map: "valid_aggmap g b f m X"
+  and finite: "finite X"
+  and in_map: "k \<in> Mapping.keys m"
+  shows "flatten_multiset (group_multiset k b f X) \<noteq> []"
+proof -
+  define M where "M = group_multiset k b f X"
+  obtain c where c_def: "ID ccompare = Some (c :: (event_data \<times> enat) comparator)" 
+    by (simp add: ID_def ccompare_prod_def ccompare_event_data_def ccompare_enat_def split:if_splits option.splits)
+  note c = ID_ccompare'[OF c_def] 
+  note c_class = comparator.linorder[OF c]
+  define M_list where "M_list = linorder.sorted_list_of_set (le_of_comp c) M"
+  obtain elem where elem_prop: "elem \<in> X \<and> drop b elem = k" using in_map valid_map imageE[of k "drop b" X] by (auto simp: valid_aggmap_def)
+  then obtain m where m_prop: "(meval_trm f elem, m) \<in> M" 
+    by (auto simp: group_multiset_def Let_def valid_aggmap_def M_def) fastforce
+  define group where "group = Set.filter (\<lambda>x. meval_trm f x = meval_trm f elem) (Set.filter (\<lambda>x. drop b x = k) X)"
+  then have "elem \<in> group" using elem_prop by (auto simp: group_def)
+  moreover have finite_g: "finite group" using finite by (auto simp: group_def)
+  ultimately have "ecard group \<noteq> 0" by (auto simp:ecard_def zero_enat_def)
+  then have m_pos: "m > 0 \<and> m \<noteq> \<infinity>" 
+    using elem_prop m_prop finite_g  by (auto simp: M_def group_multiset_def Let_def group_def ecard_def)
+  then have "the_enat m > 0"
+    apply(auto simp: the_enat_def)
+    using enat_0_iff(1) by blast
+  then obtain n where n_def: "the_enat m = Suc n" using gr0_implies_Suc by auto
+  have finite_m: "finite M" using finite by (auto simp: M_def group_multiset_def Let_def)
+  then have "(meval_trm f elem, m) \<in> set (linorder.sorted_list_of_set (le_of_comp c) M)"
+    using m_prop linorder.set_sorted_list_of_set[OF c_class] by auto
+  then show ?thesis 
+    using finite_m n_def by (simp add:flatten_multiset_def csorted_list_of_set_def c_def M_def) force
+qed
+  
 lemma valid_result_maggaux_unfolded: "valid_maggaux \<lparr>aggargs_cols = cols, aggargs_n = n, aggargs_g0 = g0, aggargs_y = y, aggargs_\<omega> = \<omega>, aggargs_b = b, aggargs_f = f\<rparr> aux X
                                   \<Longrightarrow> result_maggaux \<lparr>aggargs_cols = cols, aggargs_n = n, aggargs_g0 = g0, aggargs_y = y, aggargs_\<omega> = \<omega>, aggargs_b = b, aggargs_f = f\<rparr> aux
                                     = eval_aggargs \<lparr>aggargs_cols = cols, aggargs_n = n, aggargs_g0 = g0, aggargs_y = y, aggargs_\<omega> = \<omega>, aggargs_b = b, aggargs_f = f\<rparr> X"
 proof(induction aux)
-  case(SumAux x)
-  then show ?case by auto
+  case(SumAux m)
+  then show ?case
+  proof (cases "g0 \<and> X = {}")
+    case True
+    then show ?thesis unfolding eval_aggargs_def eval_agg_def using SumAux
+      by (auto simp add: valid_aggmap_def)
+  next
+    case False
+    then have assm_map: "\<not>(g0 \<and> Mapping.keys m = {})" using valid_aggmap_empty_data[of _ b f m X] SumAux by force
+    have assm_reg: "\<not>(g0 \<and> X = {})" using False by auto
+    show ?thesis
+    proof (cases "fst \<omega> = Formula.Agg_Sum")
+      case True
+      show ?thesis
+      proof (rule set_eqI, rule iffI)
+      fix result
+      assume "result \<in> result_maggaux \<lparr>aggargs_cols = cols, aggargs_n = n, aggargs_g0 = g0, aggargs_y = y, aggargs_\<omega> = \<omega>, aggargs_b = b, aggargs_f = f\<rparr> (SumAux m)"
+      then obtain k where k_assm: "k \<in> Mapping.keys m \<and> result = (case Mapping.lookup m k of 
+                                                      Some (_, agg_sum) \<Rightarrow> k[y:=Some agg_sum]
+                                                    | None \<Rightarrow> k)" using assm_map True by auto
+      define group where "group = Set.filter (\<lambda>x. drop b x = k) X"
+      define M where "M = (\<lambda>y. (y, ecard (Set.filter (\<lambda>x. meval_trm f x = y) group))) ` meval_trm f ` group"
+      have "Mapping.lookup m k = Some (length (flatten_multiset M), foldl plus (snd \<omega>) (flatten_multiset M))" 
+        using SumAux k_assm True by (simp add: M_def group_def Let_def lookup_default_def valid_aggmap_def group_multiset_def)
+      then have "result = k[y:= Some (eval_agg_op \<omega> M)]" 
+        using k_assm True by auto (metis eval_agg_op.simps(4) prod.collapse)
+      then show "result \<in> eval_aggargs \<lparr>aggargs_cols = cols, aggargs_n = n, aggargs_g0 = g0, aggargs_y = y, aggargs_\<omega> = \<omega>, aggargs_b = b, aggargs_f = f\<rparr> X"
+        using k_assm SumAux by (auto simp add: M_def group_def Let_def eval_agg_def eval_aggargs_def valid_aggmap_def)
+    next
+      fix result
+      assume "result \<in> eval_aggargs \<lparr>aggargs_cols = cols, aggargs_n = n, aggargs_g0 = g0, aggargs_y = y, aggargs_\<omega> = \<omega>, aggargs_b = b, aggargs_f = f\<rparr> X"
+      then obtain k where k_assm: "(k \<in> (drop b) ` X \<and> result = (let group = Set.filter (\<lambda>x. drop b x = k) X;
+                                                                   M = (\<lambda>y. (y, ecard (Set.filter (\<lambda>x. meval_trm f x = y) group))) ` meval_trm f ` group
+                                                                 in k[y:=Some (eval_agg_op \<omega> M)]))" 
+        unfolding eval_aggargs_def eval_agg_def empty_table_def using False by auto
+      define group where "group = Set.filter (\<lambda>x. drop b x = k) X"
+      define M where "M = (\<lambda>y. (y, ecard (Set.filter (\<lambda>x. meval_trm f x = y) group))) ` meval_trm f ` group"
+      have key_in_map: "k \<in> Mapping.keys m"
+        using SumAux by (auto simp add:valid_aggmap_def) (metis k_assm)
+      then have "Mapping.lookup m k = Some (length (flatten_multiset M), foldl plus (snd \<omega>) (flatten_multiset M))"
+        using SumAux True by (simp add: M_def group_def Let_def lookup_default_def valid_aggmap_def group_multiset_def)
+      then have "result = (case Mapping.lookup m k of 
+                            Some (_, agg_sum) \<Rightarrow> k[y:=Some agg_sum]
+                          | None \<Rightarrow> k)"
+        using True k_assm unfolding M_def group_def by auto (metis (no_types, lifting) eval_agg_op.simps(4) prod.exhaust_sel)
+      then show  "result \<in> result_maggaux \<lparr>aggargs_cols = cols, aggargs_n = n, aggargs_g0 = g0, aggargs_y = y, aggargs_\<omega> = \<omega>, aggargs_b = b, aggargs_f = f\<rparr> (SumAux m)"
+        using key_in_map True by auto
+    qed
+    next
+      case False
+      then have agg_type: "fst \<omega> = Formula.Agg_Avg" using SumAux by auto
+      obtain aux where aux_def: "\<omega> = (Formula.Agg_Avg, aux)" using agg_type 
+        by (simp add: prod_eq_iff)
+      show ?thesis 
+      proof (rule set_eqI, rule iffI)
+      fix result
+      assume "result \<in> result_maggaux \<lparr>aggargs_cols = cols, aggargs_n = n, aggargs_g0 = g0, aggargs_y = y, aggargs_\<omega> = \<omega>, aggargs_b = b, aggargs_f = f\<rparr> (SumAux m)"
+      then obtain k where k_assm: "k \<in> Mapping.keys m \<and> result = (case Mapping.lookup m k of 
+                                                      Some (cnt, agg_sum) \<Rightarrow> k[y:=Some (EFloat ((double_of_event_data agg_sum) / (double_of_int cnt)))]
+                                                    | None \<Rightarrow> k)" using assm_map agg_type by auto
+      define group where "group = Set.filter (\<lambda>x. drop b x = k) X"
+      define M where "M = (\<lambda>y. (y, ecard (Set.filter (\<lambda>x. meval_trm f x = y) group))) ` meval_trm f ` group"
+      have not_empty: "flatten_multiset M \<noteq> []" 
+        using flatten_multiset_not_empty[of _ b f m X k] SumAux k_assm False 
+        by (auto simp: Let_def M_def group_multiset_def group_def)
+      have "Mapping.lookup m k = Some (length (flatten_multiset M), foldl plus (EInt 0) (flatten_multiset M))" 
+        using SumAux k_assm agg_type by (simp add: M_def group_def Let_def lookup_default_def valid_aggmap_def group_multiset_def)
+      then have "result = k[y:= Some (eval_agg_op \<omega> M)]" 
+        using k_assm agg_type not_empty SumAux aux_def
+        by(auto simp add:valid_aggmap_def Let_def M_def group_def group_multiset_def split:list.splits)
+      then show "result \<in> eval_aggargs \<lparr>aggargs_cols = cols, aggargs_n = n, aggargs_g0 = g0, aggargs_y = y, aggargs_\<omega> = \<omega>, aggargs_b = b, aggargs_f = f\<rparr> X"
+        using k_assm SumAux by (auto simp add: M_def group_def Let_def eval_agg_def eval_aggargs_def valid_aggmap_def)
+    next
+      fix result
+      assume "result \<in> eval_aggargs \<lparr>aggargs_cols = cols, aggargs_n = n, aggargs_g0 = g0, aggargs_y = y, aggargs_\<omega> = \<omega>, aggargs_b = b, aggargs_f = f\<rparr> X"
+      then obtain k where k_assm: "(k \<in> (drop b) ` X \<and> result = (let group = Set.filter (\<lambda>x. drop b x = k) X;
+                                                                   M = (\<lambda>y. (y, ecard (Set.filter (\<lambda>x. meval_trm f x = y) group))) ` meval_trm f ` group
+                                                                 in k[y:=Some (eval_agg_op \<omega> M)]))" 
+        unfolding eval_aggargs_def eval_agg_def empty_table_def using assm_reg by auto
+      define group where "group = Set.filter (\<lambda>x. drop b x = k) X"
+      define M where "M = (\<lambda>y. (y, ecard (Set.filter (\<lambda>x. meval_trm f x = y) group))) ` meval_trm f ` group"
+      have "k \<in> Mapping.keys m" using k_assm SumAux 
+      by (metis (no_types, lifting) aggaux.simps(27) valid_aggmap_def valid_maggaux.simps)
+      then have not_empty: "flatten_multiset M \<noteq> []" 
+        using flatten_multiset_not_empty[of _ b f m X k] SumAux k_assm False 
+        unfolding group_multiset_def Let_def M_def group_def by fastforce
+      have key_in_map: "k \<in> Mapping.keys m"
+        using SumAux by (auto simp add:valid_aggmap_def) (metis k_assm)
+      then have "Mapping.lookup m k = Some (length (flatten_multiset M), foldl plus (EInt 0) (flatten_multiset M))"
+        using SumAux False by (simp add: M_def group_def Let_def lookup_default_def valid_aggmap_def group_multiset_def)
+      then have "result = (case Mapping.lookup m k of 
+                             Some (cnt, agg_sum) \<Rightarrow> k[y:=Some (EFloat ((double_of_event_data agg_sum) / (double_of_int cnt)))]
+                          | None \<Rightarrow> k)"
+        using False k_assm not_empty aux_def unfolding M_def group_def 
+        by(auto simp: Let_def split:list.splits)
+      then show  "result \<in> result_maggaux \<lparr>aggargs_cols = cols, aggargs_n = n, aggargs_g0 = g0, aggargs_y = y, aggargs_\<omega> = \<omega>, aggargs_b = b, aggargs_f = f\<rparr> (SumAux m)"
+        using key_in_map False by auto
+    qed
+  qed
+qed
 next 
   case(MinAux x)
   then show ?case by auto
 next
   case(MaxAux x)
   then show ?case by auto
-next
-  case(AvgAux x)
-  then show ?case by auto
 next  
   case(MedAux x)
   then show ?case by auto
 next
-  case(CntAux x)
-  from this have valid_agg: "valid_maggaux \<lparr>aggargs_cols = cols, aggargs_n = n, aggargs_g0 = g0, aggargs_y = y, aggargs_\<omega> = \<omega>, aggargs_b = b, aggargs_f = f\<rparr> (CntAux x) X"  by auto
+  case(CntAux m)
+  have agg_type: "fst \<omega> = Formula.Agg_Cnt" using CntAux by auto
   then show ?case
   proof (cases "g0 \<and> X = {}")
     case(True)
-    then have assm: "g0 \<and> X = {}" by auto
-    have result_singleton: "result_maggaux \<lparr>aggargs_cols = cols, aggargs_n = n, aggargs_g0 = g0, aggargs_y = y, aggargs_\<omega> = \<omega>, aggargs_b = b, aggargs_f = f\<rparr> (CntAux x) = singleton_table n y (eval_agg_op \<omega> {})" 
-      using assm valid_agg by auto
-    have eval_singleton: "eval_aggargs \<lparr>aggargs_cols = cols, aggargs_n = n, aggargs_g0 = g0, aggargs_y = y, aggargs_\<omega> = \<omega>, aggargs_b = b, aggargs_f = f\<rparr> X = singleton_table n y (eval_agg_op \<omega> {})"
-      using assm unfolding eval_aggargs_def eval_agg_def by auto
-    show ?thesis using result_singleton eval_singleton by auto
+    then show ?thesis 
+      unfolding eval_aggargs_def eval_agg_def
+      using CntAux by (auto simp add: valid_aggmap_def)
+  next
     case(False)
-    then have assm: "\<not>(g0 \<and> X = {})" by auto
-    have eval_subs_result: "eval_aggargs args X \<subseteq> result_maggaux args (CntAux x)" 
-    proof - {
-      
-    }
+    then have assm_map: "\<not>(g0 \<and> Mapping.keys m = {})" using CntAux by (auto simp add: valid_aggmap_def)
+    show ?thesis
+    proof (rule set_eqI, rule iffI)
+      fix result
+      assume "result \<in> result_maggaux \<lparr>aggargs_cols = cols, aggargs_n = n, aggargs_g0 = g0, aggargs_y = y, aggargs_\<omega> = \<omega>, aggargs_b = b, aggargs_f = f\<rparr> (CntAux m)"
+      then have "\<exists>k. k \<in> Mapping.keys m \<and> result = (case Mapping.lookup m k of
+                                                      Some i \<Rightarrow> k[y:=Some (EInt (integer_of_int i))]
+                                                    | None \<Rightarrow> k)" 
+        using assm_map by auto
+      then obtain k where k_assm: "k \<in> Mapping.keys m \<and> result = (case Mapping.lookup m k of
+                                                      Some i \<Rightarrow> k[y:=Some (EInt (integer_of_int i))]
+                                                    | None \<Rightarrow> k)" by blast
+      define group where "group = Set.filter (\<lambda>x. drop b x = k) X"
+      define M where "M = (\<lambda>y. (y, ecard (Set.filter (\<lambda>x. meval_trm f x = y) group))) ` meval_trm f ` group"
+      have "Mapping.lookup m k = Some (length (flatten_multiset M))" 
+        using CntAux k_assm 
+        by (simp add: M_def group_def Let_def lookup_default_def valid_aggmap_def group_multiset_def)
+      then have "result = k[y:= Some (eval_agg_op \<omega> M)]" 
+        using k_assm agg_type 
+        by (metis eval_agg_op.simps(1) option.simps(5) prod.collapse)
+      then show "result \<in> eval_aggargs \<lparr>aggargs_cols = cols, aggargs_n = n, aggargs_g0 = g0, aggargs_y = y, aggargs_\<omega> = \<omega>, aggargs_b = b, aggargs_f = f\<rparr> X"
+        using k_assm CntAux
+        by (auto simp add: M_def group_def Let_def eval_agg_def eval_aggargs_def valid_aggmap_def)
+    next
+      fix result
+      assume "result \<in> eval_aggargs \<lparr>aggargs_cols = cols, aggargs_n = n, aggargs_g0 = g0, aggargs_y = y, aggargs_\<omega> = \<omega>, aggargs_b = b, aggargs_f = f\<rparr> X"
+      then have "\<exists>k. (k \<in> (drop b) ` X \<and> result = (let group = Set.filter (\<lambda>x. drop b x = k) X;
+                                                     M = (\<lambda>y. (y, ecard (Set.filter (\<lambda>x. meval_trm f x = y) group))) ` meval_trm f ` group
+                                                   in k[y:=Some (eval_agg_op \<omega> M)]))" 
+        unfolding eval_aggargs_def eval_agg_def empty_table_def
+        using False by auto
+      then obtain k where k_assm: "(k \<in> (drop b) ` X \<and> result = (let group = Set.filter (\<lambda>x. drop b x = k) X;
+                                                                   M = (\<lambda>y. (y, ecard (Set.filter (\<lambda>x. meval_trm f x = y) group))) ` meval_trm f ` group
+                                                                 in k[y:=Some (eval_agg_op \<omega> M)]))" by blast
+      define group where "group = Set.filter (\<lambda>x. drop b x = k) X"
+      define M where "M = (\<lambda>y. (y, ecard (Set.filter (\<lambda>x. meval_trm f x = y) group))) ` meval_trm f ` group"
+      have key_in_map: "k \<in> Mapping.keys m"
+        using CntAux k_assm by (auto simp add:valid_aggmap_def)
+      then have "Mapping.lookup m k = Some (length (flatten_multiset M))"
+        using CntAux 
+        by (simp add: M_def group_def Let_def lookup_default_def valid_aggmap_def group_multiset_def)
+      then have "result = (case Mapping.lookup m k of
+                             Some i \<Rightarrow> k[y:=Some (EInt (integer_of_int i))]
+                           | None \<Rightarrow> k)"
+        using agg_type k_assm
+        unfolding M_def group_def
+        by (metis (no_types, lifting) eval_agg_op.simps(1) option.simps(5) prod.collapse)
+      then show  "result \<in> result_maggaux \<lparr>aggargs_cols = cols, aggargs_n = n, aggargs_g0 = g0, aggargs_y = y, aggargs_\<omega> = \<omega>, aggargs_b = b, aggargs_f = f\<rparr> (CntAux m)"
+        using key_in_map by auto
+    qed
+  qed
+qed
+
+lemma valid_result_maggaux: "valid_maggaux args aux X \<Longrightarrow> result_maggaux args aux = eval_aggargs args X"
+  using valid_result_maggaux_unfolded by (cases args) fast
 
 end
